type checker needs another revamp

theories/type_checker.v
@@ -8,14 +8,13 @@ Set Implicit Arguments.
 Unset Strict Implicit.
 Unset Printing Implicit Defensive.
 
-Section Host.
-
-Context `{hfc: host_function_class}.
-
-Inductive checker_type : Type :=
 (* flag for unreachable. Operand stack is represented in reverse direction (stack) *)
-| CT_type : seq value_type -> bool -> checker_type
-| CT_error : checker_type.
+Record checker_type: Type :=
+  { CT_type: list value_type;
+    CT_unr: bool;
+  }.
+
+Notation "<< ts , unr >>" := (Build_checker_type ts unr) (at level 5).
 
 Definition checker_type_eq_dec : forall v1 v2 : checker_type, {v1 = v2} + {v1 <> v2}.
 Proof. decidable_equality. Defined.
@@ -27,96 +26,75 @@ Definition eqchecker_typeP : Equality.axiom checker_type_eqb :=
 Canonical Structure checker_type_eqMixin := EqMixin eqchecker_typeP.
 Canonical Structure checker_type_eqType := Eval hnf in EqType checker_type checker_type_eqMixin.
 
-Fixpoint consume (ts: list value_type) (unr: bool) (cons : list value_type) : checker_type :=
+Fixpoint consume (ct: checker_type) (cons : list value_type) : option checker_type :=
   match cons with
-  | nil => CT_type ts unr
+  | nil => Some ct
   | t_cons :: cons' =>
-      match ts with
+      match ct.(CT_type) with
       | nil =>
-          match unr with
-          | true => CT_type nil true
-          | false => CT_error
+          match ct.(CT_unr) with
+          | true => Some <<nil, true>>
+          | false => None
           end
       | t :: ts' =>
           if t <t: t_cons then
-            consume ts' unr cons'
-          else CT_error
+            consume <<ts', ct.(CT_unr)>> cons'
+          else None
       end
   end.
 
 Definition produce (t1 : checker_type) (t2: list value_type) : checker_type :=
-  match t1 with
-  | CT_type ts unr =>
-      CT_type (t2 ++ ts) unr
-  | CT_error => CT_error
+  <<t2 ++ t1.(CT_type), t1.(CT_unr)>>.
+
+Definition type_update (ct : checker_type) (cons : list value_type) (prods : list value_type) : option checker_type :=
+  match consume ct cons with
+  | Some ct' => Some (produce ct' prods)
+  | None => None
   end.
 
-Definition type_update (curr_type : checker_type) (cons : list value_type) (prods : list value_type) : checker_type :=
-  match curr_type with
-  | CT_type ts unr => produce (consume ts unr cons) prods
-  | CT_error => CT_error
+Definition type_update_top (ct : checker_type) (cons : list value_type) (prods : list value_type) : option checker_type :=
+  match consume ct cons with
+  | Some _ => Some <<prods, true>>
+  | None => None
   end.
 
-Definition type_update_top (curr_type : checker_type) (cons : list value_type) (prods : list value_type) : checker_type :=
-  match curr_type with
-  | CT_type ts unr =>
-      match consume ts unr cons with
-      | CT_type _ _ => CT_type prods true
-      | CT_error => CT_error
-      end
-  | CT_error => CT_error
-  end.
-
-Definition type_update_select (ct : checker_type) (ots: option (list value_type)) : checker_type :=
+Definition type_update_select (ct : checker_type) (ots: option (list value_type)) : option checker_type :=
   match ots with
   | Some [::vt] => type_update ct ([:: T_num T_i32; vt; vt]) [::vt]
-  | Some _ => CT_error
+  | Some _ => None
   | None =>
-      match ct with
-      | CT_type ts unr =>
-          match ts with
-          | [:: t1; t2] =>
-              if (is_numeric_type t2) && unr then
-                CT_type [::t2] true
-              else CT_error
-          | t1 :: t2 :: t3 :: _ =>
-              if (is_numeric_type t2) && (t2 == t3) then
-                type_update ct [::T_num T_i32; t2; t3] [::t2]
-              else CT_error
-          | _ => type_update ct [::T_num T_i32] [::T_bot]
-          end
-      | CT_error => CT_error
+      match ct.(CT_type) with
+      | [:: t1; t2] =>
+          if (is_numeric_type t2) && ct.(CT_unr) then Some <<[::t2], true>>
+          else None
+      | t1 :: t2 :: t3 :: _ =>
+          if (is_numeric_type t2) && (t2 == t3) then
+            type_update ct [::T_num T_i32; t2; t3] [::t2]
+          else None
+      | _ => type_update ct [::T_num T_i32] [::T_bot]
       end
   end.
 
-Definition type_update_ref_is_null (ct : checker_type) : checker_type :=
-  match ct with
-  | CT_type ts unr =>
-      match ts with
-      | nil =>
-          if unr then
-            CT_type [::T_num T_i32] true
-          else CT_error
-      | t :: ts' =>
-          if is_ref_t t then
-            CT_type (T_num T_i32 :: ts') unr
-          else CT_error
-      end
-  | CT_error => CT_error
+Definition type_update_ref_is_null (ct : checker_type) : option checker_type :=
+  match ct.(CT_type) with
+  | nil =>
+      if ct.(CT_unr) then
+        Some <<[::T_num T_i32], true>>
+      else None
+  | t :: ts' =>
+      if is_ref_t t then
+        Some <<(T_num T_i32 :: ts'), ct.(CT_unr)>>
+      else None
   end.
 
-Definition type_update_drop (ct : checker_type) : checker_type :=
-  match ct with
-  | CT_type ts unr =>
-      match ts with
-      | nil =>
-          if unr then
-            CT_type nil true
-          else CT_error
-      | t :: ts' =>
-          CT_type ts' unr
-      end
-  | CT_error => CT_error
+Definition type_update_drop (ct : checker_type) : option checker_type :=
+  match ct.(CT_type) with
+  | nil =>
+      if ct.(CT_unr) then
+        Some <<nil, true>>
+      else None
+  | t :: ts' =>
+      Some <<ts', ct.(CT_unr)>>
   end.
 
 Fixpoint same_lab_h (iss : seq tableidx) (lab_c : seq (seq value_type)) (ts : seq value_type) : option (seq value_type) :=
@@ -146,290 +124,299 @@ Definition same_lab (iss : seq tableidx) (lab_c : seq (seq value_type)) : option
   end.
 
 Definition c_types_agree (ct : checker_type) (ts' : seq value_type) : bool :=
-  match ct with
-  | CT_type ts false => ts <ts: ts'
-  | CT_type ts true => ts <ts: (take (size ts) ts')
-  | CT_error => false
+  match ct.(CT_unr) with
+  | false => ct.(CT_type) <ts: ts'
+  | true => ct.(CT_type) <ts: (take (size ct.(CT_type)) ts')
   end.
 
 (* Using an auxiliary context with all locals/labels/returns reversed for optimisation, avoiding excessive reversing during execution *)
-Fixpoint check_single (C : t_context) (ts : checker_type) (be : basic_instruction) : checker_type :=
+Fixpoint check_single (C : t_context) (ct : option checker_type) (be : basic_instruction) : option checker_type :=
   let b_e_type_checker (C : t_context) (es : list basic_instruction) (tf : function_type) : bool :=
     let: (Tf tn tm) := tf in
-      c_types_agree (List.fold_left (check_single C) es (CT_type tn false)) tm 
-in
-  if ts == CT_error then CT_error
-  else
-  match be with
-  | BI_const_num v => type_update ts [::] [::T_num (typeof_num v)]
-  | BI_const_vec v => type_update ts [::] [::T_vec (typeof_vec v)]
-  | BI_ref_null t => type_update ts [::]  [::T_ref t]
-  | BI_ref_is_null => type_update_ref_is_null ts
-  | BI_ref_func x =>
-      match lookup_N C.(tc_funcs) x with
-      | Some _ =>
-          if x \in C.(tc_refs)
-          then type_update ts [::] [::T_ref T_funcref]
-          else CT_error
-      | _ => CT_error
-      end
-  | BI_unop t op =>
-    match op with
-    | Unop_i _ => if is_int_t t
-                  then type_update ts [::(T_num t)] [::T_num t]
-                  else CT_error
-    | Unop_f _ => if is_float_t t
-                  then type_update ts [::(T_num t)] [::T_num t]
-                  else CT_error
-    | Unop_extend _ =>
-        (* Technically, this needs to check validity of the extend arg; but such instruction can never arise from parsing *)
-                  if is_int_t t
-                  then type_update ts [::(T_num t)] [::T_num t]
-                  else CT_error
+    match List.fold_left (check_single C) es (Some <<tn, false>>) with
+    | Some ts => c_types_agree ts tm
+    | None => false
     end
-  | BI_binop t op =>
-    match op with
-    | Binop_i _ => if is_int_t t
-                  then type_update ts [::(T_num t); (T_num t)] [::(T_num t)]
-                  else CT_error
-    | Binop_f _ => if is_float_t t
-                  then type_update ts [::(T_num t); (T_num t)] [::(T_num t)]
-                  else CT_error
-    end
-  | BI_testop t _ =>
-    if is_int_t t
-    then type_update ts [::(T_num t)] [::(T_num T_i32)]
-    else CT_error
-  | BI_relop t op =>
-    match op with
-    | Relop_i _ => if is_int_t t
-                  then type_update ts [::(T_num t); (T_num t)] [::(T_num T_i32)]
-                  else CT_error
-    | Relop_f _ => if is_float_t t
-                  then type_update ts [::(T_num t); (T_num t)] [::(T_num T_i32)]
-                  else CT_error
-    end
-  | BI_cvtop t2 op t1 sx =>
-    if cvtop_valid t2 op t1 sx
-    then type_update ts [::(T_num t1)] [::(T_num t2)]
-    else CT_error
-  | BI_unreachable => CT_type nil true
-  | BI_nop => ts
-  | BI_drop => type_update_drop ts
-  | BI_select ot => type_update_select ts ot
-  | BI_block bt es =>
-      match expand_t C bt with
-      | Some (Tf tn tm) =>
-          if b_e_type_checker (upd_label C ([::tm] ++ tc_labels C)) es (Tf tn tm)
-          then type_update ts (tn) tm
-          else CT_error
-      | None => CT_error
-      end
-  | BI_loop bt es =>
-      match expand_t C bt with
-      | Some (Tf tn tm) =>
-          if b_e_type_checker (upd_label C ([::tn] ++ tc_labels C)) es (Tf tn tm)
-          then type_update ts (tn) tm
-          else CT_error
-      | None => CT_error
-      end
-  | BI_if bt es1 es2 =>
-      match expand_t C bt with
-      | Some (Tf tn tm) =>
-          if b_e_type_checker (upd_label C ([::tm] ++ tc_labels C)) es1 (Tf tn tm)
-             && b_e_type_checker (upd_label C ([::tm] ++ tc_labels C)) es2 (Tf tn tm)
-          then type_update ts ((T_num T_i32 :: tn)) tm
-          else CT_error
-      | None => CT_error
-      end
-  | BI_br i =>
-      match lookup_N (tc_labels C) i with
-      | Some xx => type_update_top ts (xx) nil
-      | None => CT_error 
-      end
-  | BI_br_if i =>
-      match lookup_N (tc_labels C) i with
-      | Some xx => type_update ts ((T_num T_i32 :: xx)) xx
-      | None => CT_error 
-      end
-  | BI_br_table iss i =>
-    match same_lab (iss ++ [::i]) (tc_labels C) with
-    | None => CT_error
-    | Some tls => type_update_top ts ((T_num T_i32 :: tls)) nil
-    end
-  | BI_return =>
-    match tc_return C with
-    | None => CT_error
-    | Some tls => type_update_top ts (tls) nil
-    end
-  | BI_call x =>
-      match lookup_N (tc_funcs C) x with
-      | None => CT_error 
-      | Some (Tf tn tm) =>
-          type_update ts (tn) tm
-      end
-  | BI_call_indirect x y =>
-      match lookup_N C.(tc_tables) x with
-      | Some tabt =>
-          if tabt.(tt_elem_type) == T_funcref then
-            match lookup_N (tc_types C) y with
-            | Some (Tf tn tm) =>
-                type_update ts ((T_num T_i32 :: tn)) tm
-            | None => CT_error 
-            end
-          else CT_error
-      | None => CT_error
-      end
-  | BI_local_get i =>
-      match lookup_N (tc_locals C) i with
-      | None => CT_error 
-      | Some xx => type_update ts [::] [::xx]
-      end
-  | BI_local_set i =>
-      match lookup_N (tc_locals C) i with
-      | None => CT_error 
-      | Some xx => type_update ts [::xx] [::]
-      end
-  | BI_local_tee i =>
-      match lookup_N (tc_locals C) i with
-      | None => CT_error 
-      | Some xx => type_update ts [::xx] [::xx]
-      end
-  | BI_global_get i =>
-      match lookup_N (tc_globals C) i with
-      | None => CT_error 
-      | Some xx => type_update ts [::] [::tg_t xx]
-      end
-  | BI_global_set i =>
-      match lookup_N (tc_globals C) i with
-      | None => CT_error 
-      | Some xx =>
-          if is_mut xx
-          then type_update ts [::(tg_t xx)] [::]
-          else CT_error
-      end
-  | BI_table_get x =>
-      match lookup_N (tc_tables C) x with
-      | None => CT_error 
-      | Some tabt =>
-          type_update ts [::(T_num T_i32)] [::T_ref tabt.(tt_elem_type)]
-      end
-  | BI_table_set x =>
-      match lookup_N (tc_tables C) x with
-      | None => CT_error 
-      | Some tabt =>
-          type_update ts [::(T_ref tabt.(tt_elem_type)); (T_num T_i32)] nil
-      end
-  | BI_table_size x =>
-      match lookup_N (tc_tables C) x with
-      | None => CT_error 
-      | Some tabt =>
-          type_update ts nil [::T_num T_i32]
-      end
-  | BI_table_grow x =>
-      match lookup_N (tc_tables C) x with
-      | None => CT_error 
-      | Some tabt =>
-          type_update ts [::T_num T_i32; (T_ref tabt.(tt_elem_type))] [::T_num T_i32]
-      end
-  | BI_table_fill x =>
-      match lookup_N (tc_tables C) x with
-      | None => CT_error 
-      | Some tabt =>
-          type_update ts [::(T_num T_i32); (T_ref tabt.(tt_elem_type)); (T_num T_i32)] nil
-      end
-  | BI_table_copy x y =>
-      match lookup_N (tc_tables C) x with
-      | None => CT_error 
-      | Some tabt1 =>
-          match lookup_N (tc_tables C) y with
-          | Some tabt2 =>
-              if tabt1.(tt_elem_type) == tabt2.(tt_elem_type)
-              then type_update ts [::(T_num T_i32); (T_num T_i32); (T_num T_i32)] nil
-              else CT_error
-          | None => CT_error
+  in
+  match ct with
+  | None => None
+  | Some ts =>
+      match be with
+      | BI_const_num v => type_update ts [::] [::T_num (typeof_num v)]
+      | BI_const_vec v => type_update ts [::] [::T_vec (typeof_vec v)]
+      | BI_ref_null t => type_update ts [::]  [::T_ref t]
+      | BI_ref_is_null => type_update_ref_is_null ts
+      | BI_ref_func x =>
+          match lookup_N C.(tc_funcs) x with
+          | Some _ =>
+              if x \in C.(tc_refs)
+              then type_update ts [::] [::T_ref T_funcref]
+              else None
+          | _ => None
           end
-      end
-  | BI_table_init x y =>
-      match lookup_N (tc_tables C) x with
-      | None => CT_error 
-      | Some tabt =>
-          match lookup_N (tc_elems C) y with
-          | Some t =>
-              if tabt.(tt_elem_type) == t
-              then type_update ts [::(T_num T_i32); (T_num T_i32); (T_num T_i32)] nil
-              else CT_error
-          | None => CT_error
+      | BI_unop t op =>
+          match op with
+          | Unop_i _ => if is_int_t t
+                       then type_update ts [::(T_num t)] [::T_num t]
+                       else None
+          | Unop_f _ => if is_float_t t
+                       then type_update ts [::(T_num t)] [::T_num t]
+                       else None
+          | Unop_extend _ =>
+              (* Technically, this needs to check validity of the extend arg; but such instruction can never arise from parsing *)
+              if is_int_t t
+              then type_update ts [::(T_num t)] [::T_num t]
+              else None
           end
-      end
-  | BI_elem_drop x =>
-      match lookup_N (tc_elems C) x with
-      | None => CT_error 
-      | Some tabt => ts
-      end
-  | BI_load t tp_sx a off =>
-      match lookup_N C.(tc_mems) 0%N with
-      | Some _ =>
-          if load_store_t_bounds a (option_projl tp_sx) t
-          then type_update ts [::(T_num T_i32)] [::T_num t]
-          else CT_error
-      | None => CT_error
-      end
-  | BI_store t tp a off =>
-      match lookup_N C.(tc_mems) 0%N with
-      | Some _ =>
-          if load_store_t_bounds a tp t
-          then type_update ts [::T_num t; T_num T_i32] [::]
-          else CT_error
-      | None => CT_error
-      end
-  | BI_memory_size =>
-      match lookup_N C.(tc_mems) 0%N with
-      | Some _ =>
-          type_update ts [::] [::(T_num T_i32)]
-      | None => CT_error
-      end
-  | BI_memory_grow =>
-      match lookup_N C.(tc_mems) 0%N with
-      | Some _ =>
-          type_update ts [::(T_num T_i32)] [::(T_num T_i32)]
-      | None => CT_error
-      end
-  | BI_memory_fill =>
-      match lookup_N C.(tc_mems) 0%N with
-      | Some _ =>
-          type_update ts [::(T_num T_i32); (T_num T_i32); (T_num T_i32)] nil
-      | None => CT_error
-      end
-  | BI_memory_copy =>
-      match lookup_N C.(tc_mems) 0%N with
-      | Some _ =>
-          type_update ts [::(T_num T_i32); (T_num T_i32); (T_num T_i32)] nil
-      | None => CT_error
-      end
-  | BI_memory_init x =>
-      match lookup_N C.(tc_mems) 0%N with
-      | Some _ =>
-          match lookup_N C.(tc_datas) x with
+      | BI_binop t op =>
+          match op with
+          | Binop_i _ => if is_int_t t
+                        then type_update ts [::(T_num t); (T_num t)] [::(T_num t)]
+                        else None
+          | Binop_f _ => if is_float_t t
+                        then type_update ts [::(T_num t); (T_num t)] [::(T_num t)]
+                        else None
+          end
+      | BI_testop t _ =>
+          if is_int_t t
+          then type_update ts [::(T_num t)] [::(T_num T_i32)]
+          else None
+      | BI_relop t op =>
+          match op with
+          | Relop_i _ => if is_int_t t
+                        then type_update ts [::(T_num t); (T_num t)] [::(T_num T_i32)]
+                        else None
+          | Relop_f _ => if is_float_t t
+                        then type_update ts [::(T_num t); (T_num t)] [::(T_num T_i32)]
+                        else None
+          end
+      | BI_cvtop t2 op t1 sx =>
+          if cvtop_valid t2 op t1 sx
+          then type_update ts [::(T_num t1)] [::(T_num t2)]
+          else None
+      | BI_unreachable => Some <<nil, true>>
+      | BI_nop => Some ts
+      | BI_drop => type_update_drop ts
+      | BI_select ot => type_update_select ts ot
+      | BI_block bt es =>
+          match expand_t C bt with
+          | Some (Tf tn tm) =>
+              if b_e_type_checker (upd_label C ([::tm] ++ tc_labels C)) es (Tf tn tm)
+              then type_update ts (tn) tm
+              else None
+          | None => None
+          end
+      | BI_loop bt es =>
+          match expand_t C bt with
+          | Some (Tf tn tm) =>
+              if b_e_type_checker (upd_label C ([::tn] ++ tc_labels C)) es (Tf tn tm)
+              then type_update ts (tn) tm
+              else None
+          | None => None
+          end
+      | BI_if bt es1 es2 =>
+          match expand_t C bt with
+          | Some (Tf tn tm) =>
+              if b_e_type_checker (upd_label C ([::tm] ++ tc_labels C)) es1 (Tf tn tm)
+                 && b_e_type_checker (upd_label C ([::tm] ++ tc_labels C)) es2 (Tf tn tm)
+              then type_update ts ((T_num T_i32 :: tn)) tm
+              else None
+          | None => None
+          end
+      | BI_br i =>
+          match lookup_N (tc_labels C) i with
+          | Some xx => type_update_top ts (xx) nil
+          | None => None 
+          end
+      | BI_br_if i =>
+          match lookup_N (tc_labels C) i with
+          | Some xx => type_update ts ((T_num T_i32 :: xx)) xx
+          | None => None 
+          end
+      | BI_br_table iss i =>
+          match same_lab (iss ++ [::i]) (tc_labels C) with
+          | None => None
+          | Some tls => type_update_top ts ((T_num T_i32 :: tls)) nil
+          end
+      | BI_return =>
+          match tc_return C with
+          | None => None
+          | Some tls => type_update_top ts (tls) nil
+          end
+      | BI_call x =>
+          match lookup_N (tc_funcs C) x with
+          | None => None 
+          | Some (Tf tn tm) =>
+              type_update ts (tn) tm
+          end
+      | BI_call_indirect x y =>
+          match lookup_N C.(tc_tables) x with
+          | Some tabt =>
+              if tabt.(tt_elem_type) == T_funcref then
+                match lookup_N (tc_types C) y with
+                | Some (Tf tn tm) =>
+                    type_update ts ((T_num T_i32 :: tn)) tm
+                | None => None 
+                end
+              else None
+          | None => None
+          end
+      | BI_local_get i =>
+          match lookup_N (tc_locals C) i with
+          | None => None 
+          | Some xx => type_update ts [::] [::xx]
+          end
+      | BI_local_set i =>
+          match lookup_N (tc_locals C) i with
+          | None => None 
+          | Some xx => type_update ts [::xx] [::]
+          end
+      | BI_local_tee i =>
+          match lookup_N (tc_locals C) i with
+          | None => None 
+          | Some xx => type_update ts [::xx] [::xx]
+          end
+      | BI_global_get i =>
+          match lookup_N (tc_globals C) i with
+          | None => None 
+          | Some xx => type_update ts [::] [::tg_t xx]
+          end
+      | BI_global_set i =>
+          match lookup_N (tc_globals C) i with
+          | None => None 
+          | Some xx =>
+              if is_mut xx
+              then type_update ts [::(tg_t xx)] [::]
+              else None
+          end
+      | BI_table_get x =>
+          match lookup_N (tc_tables C) x with
+          | None => None 
+          | Some tabt =>
+              type_update ts [::(T_num T_i32)] [::T_ref tabt.(tt_elem_type)]
+          end
+      | BI_table_set x =>
+          match lookup_N (tc_tables C) x with
+          | None => None 
+          | Some tabt =>
+              type_update ts [::(T_ref tabt.(tt_elem_type)); (T_num T_i32)] nil
+          end
+      | BI_table_size x =>
+          match lookup_N (tc_tables C) x with
+          | None => None 
+          | Some tabt =>
+              type_update ts nil [::T_num T_i32]
+          end
+      | BI_table_grow x =>
+          match lookup_N (tc_tables C) x with
+          | None => None 
+          | Some tabt =>
+              type_update ts [::T_num T_i32; (T_ref tabt.(tt_elem_type))] [::T_num T_i32]
+          end
+      | BI_table_fill x =>
+          match lookup_N (tc_tables C) x with
+          | None => None 
+          | Some tabt =>
+              type_update ts [::(T_num T_i32); (T_ref tabt.(tt_elem_type)); (T_num T_i32)] nil
+          end
+      | BI_table_copy x y =>
+          match lookup_N (tc_tables C) x with
+          | None => None 
+          | Some tabt1 =>
+              match lookup_N (tc_tables C) y with
+              | Some tabt2 =>
+                  if tabt1.(tt_elem_type) == tabt2.(tt_elem_type)
+                  then type_update ts [::(T_num T_i32); (T_num T_i32); (T_num T_i32)] nil
+                  else None
+              | None => None
+              end
+          end
+      | BI_table_init x y =>
+          match lookup_N (tc_tables C) x with
+          | None => None 
+          | Some tabt =>
+              match lookup_N (tc_elems C) y with
+              | Some t =>
+                  if tabt.(tt_elem_type) == t
+                  then type_update ts [::(T_num T_i32); (T_num T_i32); (T_num T_i32)] nil
+                  else None
+              | None => None
+              end
+          end
+      | BI_elem_drop x =>
+          match lookup_N (tc_elems C) x with
+          | None => None 
+          | Some tabt => Some ts
+          end
+      | BI_load t tp_sx a off =>
+          match lookup_N C.(tc_mems) 0%N with
+          | Some _ =>
+              if load_store_t_bounds a (option_projl tp_sx) t
+              then type_update ts [::(T_num T_i32)] [::T_num t]
+              else None
+          | None => None
+          end
+      | BI_store t tp a off =>
+          match lookup_N C.(tc_mems) 0%N with
+          | Some _ =>
+              if load_store_t_bounds a tp t
+              then type_update ts [::T_num t; T_num T_i32] [::]
+              else None
+          | None => None
+          end
+      | BI_memory_size =>
+          match lookup_N C.(tc_mems) 0%N with
+          | Some _ =>
+              type_update ts [::] [::(T_num T_i32)]
+          | None => None
+          end
+      | BI_memory_grow =>
+          match lookup_N C.(tc_mems) 0%N with
+          | Some _ =>
+              type_update ts [::(T_num T_i32)] [::(T_num T_i32)]
+          | None => None
+          end
+      | BI_memory_fill =>
+          match lookup_N C.(tc_mems) 0%N with
           | Some _ =>
               type_update ts [::(T_num T_i32); (T_num T_i32); (T_num T_i32)] nil
-          | None => CT_error
+          | None => None
           end
-      | None => CT_error
-      end
-  | BI_data_drop x =>
-      match lookup_N C.(tc_datas) x with
-      | Some _ => ts
-      | None => CT_error
+      | BI_memory_copy =>
+          match lookup_N C.(tc_mems) 0%N with
+          | Some _ =>
+              type_update ts [::(T_num T_i32); (T_num T_i32); (T_num T_i32)] nil
+          | None => None
+          end
+      | BI_memory_init x =>
+          match lookup_N C.(tc_mems) 0%N with
+          | Some _ =>
+              match lookup_N C.(tc_datas) x with
+              | Some _ =>
+                  type_update ts [::(T_num T_i32); (T_num T_i32); (T_num T_i32)] nil
+              | None => None
+              end
+          | None => None
+          end
+      | BI_data_drop x =>
+          match lookup_N C.(tc_datas) x with
+          | Some _ => Some ts
+          | None => None
+          end
       end
   end.
 
-Definition check (C : t_context) (es : list basic_instruction) (ts : checker_type): checker_type :=
-  List.fold_left (check_single C) es ts.
+
+Definition check (C : t_context) (es : list basic_instruction) (ct : option checker_type): option checker_type :=
+  List.fold_left (check_single C) es ct.
 
 Definition b_e_type_checker_aux (C : t_context) (es : list basic_instruction) (tf : function_type) : bool :=
   let: (Tf tn tm) := tf in
-  c_types_agree (List.fold_left (check_single C) es (CT_type tn false)) tm.
+  match (List.fold_left (check_single C) es (Some <<tn, false>>)) with
+  | Some ts =>
+      c_types_agree ts tm
+  | None => false
+  end.
 
 (*
   A context with local/label/return reversed for optimised validation.
@@ -458,5 +445,3 @@ Definition context_reverse (C: t_context): t_context :=
 Definition b_e_type_checker (C : t_context) (es : list basic_instruction) (tf : function_type) : bool :=
   let: (Tf tn tm) := tf in
   b_e_type_checker_aux (context_reverse C) es (Tf (rev tn) (rev tm)).
-
-End Host.
